proof/access-control/ARM/ArchAccess.thy
@@ -88,6 +88,11 @@ lemmas state_vrefs_upd =
   revokable_update.state_vrefs
   machine_state_update.state_vrefs
   more_update.state_vrefs
+  scheduler_action_update.state_vrefs
+  domain_index_update.state_vrefs
+  cur_domain_update.state_vrefs
+  domain_time_update.state_vrefs
+  ready_queues_update.state_vrefs
 
 end
 
@@ -138,6 +143,7 @@ abbreviation integrity_asids_aux ::
      pp_opt = pp_opt' \<or> (\<forall>asid'. asid' \<noteq> 0 \<and> asid_high_bits_of asid' = asid_high_bits_of asid
                                  \<longrightarrow> pasASIDAbs aag asid' \<in> subjects)"
 
+\<comment> \<open>FIXME: could we define integrity_asids to operate on arch_state only?\<close>
 definition integrity_asids ::
   "'a PAS \<Rightarrow> 'a set \<Rightarrow> obj_ref \<Rightarrow> asid \<Rightarrow> 'y::state_ext state \<Rightarrow> 'z:: state_ext state  \<Rightarrow> bool" where
   "integrity_asids aag subjects x a s s' \<equiv>
@@ -159,6 +165,11 @@ lemmas integrity_asids_updates =
   interrupt_update.integrity_asids_update
   cur_thread_update.integrity_asids_update
   machine_state_update.integrity_asids_update
+  scheduler_action_update.integrity_asids_update
+  domain_index_update.integrity_asids_update
+  cur_domain_update.integrity_asids_update
+  domain_time_update.integrity_asids_update
+  ready_queues_update.integrity_asids_update
 
 (* The kheap isn't used in ARM's integrity_asids definition,
    but we need the following lemmas in some generic contexts *)
